Progress on safety proof

linking/safety.v
@@ -2,11 +2,32 @@ Require Import ssreflect ssrbool ssrnat ssrfun eqtype seq fintype finfun.
 Set Implicit Arguments.
 Unset Strict Implicit.
 
+Require Import msl.Coqlib2.
+
+Require Import Integers.
+
 Require Import juicy_mem.
 Require Import juicy_extspec.
 
 Require Import pos.
 Require Import linking. 
+
+Section upd_exit.
+
+Variable Z : Type.
+
+Variable spec : external_specification juicy_mem external_function Z.
+
+Definition upd_exit' (Q_exit : option val -> Z -> juicy_mem -> Prop) :=
+  {| ext_spec_type := ext_spec_type spec
+   ; ext_spec_pre := ext_spec_pre spec
+   ; ext_spec_post := ext_spec_post spec
+   ; ext_spec_exit := Q_exit |}.
+
+Definition upd_exit (ef : external_function) (x : ext_spec_type spec ef) := 
+  upd_exit' (ext_spec_post spec ef x (sig_res (ef_sig ef))).
+
+End upd_exit.
 
 Section safety.
 
@@ -16,16 +37,158 @@ Variable plt : ident -> option 'I_N.
 
 Variable sems : 'I_N -> Modsem.t juicy_mem.
 
-Notation linked := (LinkerSem.coresem N sems plt).
-
 Variable Z : Type.
 
 Variable spec : external_specification juicy_mem external_function Z.
 
 Variable ge : ge_ty.
 
-Variable all_safe : 
-  forall (entry_point : ident) idx,
-  plt entry_point = Some idx -> 
+Variable entry_points_safe : 
+  forall ef fid idx bf args z m,
+  let: tys := sig_args (ef_sig ef) in
+  let: rty := sig_res (ef_sig ef) in
+  LinkerSem.fun_id ef = Some fid -> 
+  plt fid = Some idx -> 
+  let: ge_idx := Modsem.ge (sems idx) in
+  let: sem_idx := Modsem.sem (sems idx) in
+  Genv.find_symbol ge_idx fid = Some bf -> 
+  forall x : ext_spec_type spec ef,
+  ext_spec_pre spec ef x tys args z m -> 
+  exists c, 
+    [/\ initial_core sem_idx ge_idx (Vptr bf Int.zero) args = Some c 
+      & (forall n, safeN sem_idx (upd_exit x) ge_idx n z c m)].
+
+Notation linked_sem := (LinkerSem.coresem N sems plt).
+
+Notation linked_st := (Linker.t N sems).
+
+Require Import stack.
+
+Fixpoint tail_safe (n : nat)
+    (ef : external_function) (x : ext_spec_type spec ef)
+    (efs : seq external_function) (s : Stack.t (Core.t sems)) : Prop :=
+  match efs, s with 
+    | nil, nil => True
+    | ef_top :: efs', c :: s' => 
+        let: c_idx := Core.i c in
+        let: c_c := Core.c c in 
+        let: c_sig := Core.sg c in 
+        let: c_ge := Modsem.ge (sems c_idx) in
+        let: c_sem := Modsem.sem (sems c_idx) in
+          c_sig = ef_sig ef_top /\
+          exists sig args z m (x_top : ext_spec_type spec ef_top), 
+          [/\ at_external c_sem c_c = Some (ef, sig, args) 
+            , ext_spec_pre spec ef x (sig_args sig) args z m 
+            , (forall ret z' m',
+               ext_spec_post spec ef x (sig_res sig) ret z' m' ->
+               let: spec' := @upd_exit _ spec ef_top x_top in
+               exists c', 
+               [/\ after_external c_sem ret c_c = Some c'
+                 & safeN c_sem spec' c_ge n z' c' m'])
+           & @tail_safe n ef_top x_top efs' s']
+    | _, _ => False
+  end.
+
+Definition head_safe n ef (x : ext_spec_type spec ef) (c : Core.t sems) z m :=
+  let: c_idx := Core.i c in
+  let: c_c := Core.c c in 
+  let: c_sig := Core.sg c in 
+  let: c_ge := Modsem.ge (sems c_idx) in
+  let: c_sem := Modsem.sem (sems c_idx) in
+  [/\ c_sig = ef_sig ef 
+    & safeN c_sem (@upd_exit _ spec ef x) c_ge n z c_c m].
+
+Definition stack_safe (n : nat)
+    (efs : seq external_function) (s : Stack.t (Core.t sems)) z m : Prop :=
+  match efs, s with
+    | nil, nil => True
+    | ef :: efs', c :: s' => 
+      exists x : ext_spec_type spec ef,
+      [/\ @head_safe n ef x c z m & @tail_safe n ef x efs' s']
+    | _, _ => False
+  end.
+
+Definition all_safe n z (l : linked_st) m :=
+  exists efs : list external_function, 
+    stack_safe n efs (CallStack.callStack (Linker.stack l)) z m.
+
+Lemma all_safe_inv n z l m :
+  all_safe (S n) z l m -> 
+  (exists l' m', [/\ corestep linked_sem ge l m l' m' & all_safe n z l' m'])
+  \/ (exists rv, halted linked_sem l = Some rv).
+Proof.
+case=> efs; case: l=> fn_tbl; case; case=> //= a1 l1 Hwf.
+case: efs=> // ef efs'; case=> Hx []Hhd Htl; move: Hhd; rewrite /head_safe /=.
+case Hat: (at_external _ _)=> [[[ef' sig'] args']|].
+
+{ (* at_external *)
+have ->: halted (Modsem.sem (sems (Core.i a1))) (Core.c a1) = None.
+  admit.
+admit.
+}
+case Hhlt: (halted _ _)=> [rv|].
+
+{ (* halted *)
+case=> Hsg Hexit; case: l1 Hwf Htl.
++ (* l1 = [::] *) 
+move=> Hwf; case: efs'=> // _; right; exists rv.
+rewrite /LinkerSem.halted /inContext /=.
+rewrite /LinkerSem.halted0 /peekCore /= Hhlt.
+have Hty: val_casted.val_has_type_func rv (proj_sig_res (ef_sig ef)).
+  admit.
+by rewrite Hsg Hty.
++ (* l1 = [a2 :: l2] *)
+move=> a2 l2 Hwf; case: efs'=> // ef' efs'' []Hsg' Htl.
+move: Htl; case=> sig []args []z0 []m0 []x0 []Hat0 Hpre0.
+have ->: sig_res sig = sig_res (ef_sig ef).
+  admit. (*FIXME*)
+case/(_ (Some rv) z m Hexit)=> c' []Haft0 Hsafe Htl; left.
+have Hwf': wf_callStack [:: a2 & l2].
+{ clear -Hwf; move: Hwf; rewrite /wf_callStack; case/andP=> /=.
+  by case/andP=> ? ? ?; apply/andP; split. }
+set l' := {| Linker.fn_tbl := fn_tbl
+           ; Linker.stack := CallStack.mk [:: a2 & l2] Hwf' |}.
+exists (updCore l' (Core.upd a2 c')), m; split.
+right; split=> //.
+split.
+admit. (*ncorestep*)
+rewrite /LinkerSem.at_external0 /peekCore /= Hat.
+rewrite /inContext /=.
+rewrite /LinkerSem.halted0 /peekCore /= Hhlt.
+have Hty: val_casted.val_has_type_func rv (proj_sig_res (ef_sig ef)).
+  admit.
+rewrite Hsg Hty.
+rewrite /LinkerSem.after_external /peekCore /= Haft0.
+f_equal.
+f_equal.
+apply: proof_irr.
+
+{ (* all_safe *)
+exists [:: ef' & efs''], x0; split.
+
++ (* head_safe *)
+split=> //.
+clear -Hsafe.
+move: Hsafe.
+case: a2 c'=> i c sg c'.
+rewrite /Core.upd /Core.i /Core.c.
+admit. (*by safe downward*)
+
+rewrite -/tail_safe in Htl.
+rewrite /=.
+admit. (*by tail_safe_downward*)
+}
+}
+
+{ (* corestep *)
+case=> Hsg; case=> c' []m' []Hstep Hsafe; left.
+set l := {| Linker.fn_tbl := fn_tbl
+          ; Linker.stack := CallStack.mk (a1 :: l1) Hwf |}.
+exists (updCore l (Core.upd a1 c')), m'; split.
+by left; rewrite /LinkerSem.corestep0 /peekCore; exists c'.
+exists [:: ef & efs'], Hx; split=> //; rewrite /=.
+admit. (*by tail_safe_downward*)
+}
+Qed.
 
 End safety.  
